beginning work refactoring PagedSystem

Splinter/Paged/PagedJournalMod.i.dfy
@@ -14,23 +14,10 @@ module PagedJournalMod {
   import opened StampedMapMod
   import opened MsgHistoryMod
 
-  // TODO(jonh): no wait we were not going to represent pointers at all! not at this layer.
-  // In the implementation, the PagePointer is a CU. But here we don't know
-  // about a storage, all we know is that there's some mapping from PagePointer
-  // to our pages.
-  type PagePointer(==,!new)
-  function ArbitraryPointer() : PagePointer {
-    var ptr :| true; ptr
-  }
-
-  datatype Superblock = Superblock(
-    freshestPtr: Option<PagePointer>,
-    boundaryLSN : LSN)  // exclusive: lsns <= boundaryLSN are discarded
-
   // On-disk JournalRecords
   datatype JournalRecord = JournalRecord(
     messageSeq: MsgHistory,
-    priorPtr: Option<PagePointer>   // linked list pointer
+    priorRec: Option<JournalRecord>
   )
   {
     predicate WF()
@@ -41,36 +28,34 @@ module PagedJournalMod {
       && messageSeq.MsgHistory?
     }
 
-    function priorSB(sb: Superblock) : Superblock
+    // priorSB(tj: TruncatedJournal) : TruncatedJournal
+    // ports to tj.prior()
+  }
+
+  // A TruncatedJournal is some long chain but which we ignore beyond the boundaryLSN
+  // (because we have a map telling us that part of the history).
+  // In the refinement layer below, we'll have some situations where the disk has extra
+  // journal records, but we'll ignore them in the refinement (since we never read them)
+  // and instead supply a None? for the interpretation at this layer.
+  // That's what keeps us out of trouble when those un-read pages get reclaimed -- we don't
+  // want to have to say we can interpret them.
+  datatype TruncatedJournal = TruncatedJournal(
+    freshestRec: Option<JournalRecord>,
+    boundaryLSN : LSN)  // exclusive: lsns <= boundaryLSN are discarded
+  {
+    function prior() : TruncatedJournal
+      requires freshestRec.Some?
     {
-      Superblock(priorPtr, sb.boundaryLSN)
+      TruncatedJournal(freshestRec.value.priorRec, boundaryLSN)
     }
   }
 
-  // This journal is made up of JournalRecord-typed pages, indexed by PagePointer.
-  // A Storage corresponds to the partition of the storage "owned" by the journal, and hence
-  // all of those pages hold JournalRecords.
-  // An unparseable UninterpretedPage at the level below interprets to just a
-  // missing key in this Storage map.
-  type Storage = imap<PagePointer, JournalRecord>
-  predicate AnyPointer(ptr: PagePointer)
-  {
-    true
-  }
-  predicate FullStorage(storage: Storage) {
-    forall ptr :: AnyPointer(ptr) <==> ptr in storage
-  }
-
-  function EmptyLSNMap() : map<LSN, PagePointer>
-  {
-    var empty:set<LSN> := {};
-    map lsn | lsn in empty :: ArbitraryPointer()
-  }
-
   datatype ChainResult =
-    | ChainFailed // missing blocks, or parse failures, or records that don't stitch.
+    | ChainFailed // Records that don't stitch correctly.
+      // (In the layer below, missing or unparseable blocks will interpret to None?s here,
+      // and those won't stitch.)
 
-    | ChainSuccess( // the disk had a parseable journal chain on it.
+    | ChainSuccess( // the chain stitches together.
         records: seq<JournalRecord>,
         interp: MsgHistory)
   {
@@ -79,83 +64,62 @@ module PagedJournalMod {
       && (ChainSuccess? ==> interp.WF())
     }
 
-    predicate Concatable(next: ChainResult)
+    // 'earlier' is the remainder of our linked list, which should contain earlier LSNs.
+    predicate Concatable(earlier: ChainResult)
     {
       && WF()
-      && next.WF()
-      // next has at most one record
-      && (next.ChainSuccess? ==> |next.records| <= 1)
-      // this and next both success => they have linking LSNs
-      && (&& ChainSuccess?
-          && next.ChainSuccess?
-          ==>
-          && next.interp.MsgHistory?
-          && interp.CanFollow(next.interp.seqEnd))
+      && earlier.WF()
+      // earlier has at most one record
+      && (earlier.ChainSuccess? ==> |earlier.records| <= 1)
     }
 
     // Stitch another single-record result onto this one.
-    function Concat(next: ChainResult) : ChainResult
-      requires Concatable(next)
-      ensures Concat(next).WF()
+    function Concat(earlier: ChainResult) : ChainResult
+      requires Concatable(earlier)
+      ensures Concat(earlier).WF()
     {
-      if ChainFailed? || next.ChainFailed?
+      if ChainFailed? || earlier.ChainFailed?
       then ChainFailed
-      else if 0 == |next.records|
+      else if 0 == |earlier.records|
       then this
-      else ChainSuccess(records + next.records, next.interp.Concat(interp))
-    }
-
-    function lsnMap(cu: Option<PagePointer>) : map<LSN, PagePointer>
-    {
-      if ChainFailed? || cu.None?
-      then
-        EmptyLSNMap()
-      else
-        map lsn | lsn in interp.LSNSet() :: cu.value
+      else ChainSuccess(records + earlier.records, earlier.interp.Concat(interp))
     }
   }
 
   datatype ChainLookupRow = ChainLookupRow(
-    sb: Superblock, // The bounds definition -- first PagePointer, boundaryLSN.
+    tj: TruncatedJournal,  // The bounds definition -- boundaryLSN plus the journal it bounds.
     expectedEnd: LSN,     // if hasRecord() && seqEnd != expectedEnd, rowResult.ChainFailed.
       // This is how we can have two chains, one that Successes and one that Faileds, even though
       // they're looking at the same journalRecord. Note that, if !hasRecord(), expectedEnd can
       // be anything, to satisfy the ValidSuccessorTo coming from the next row.
-    journalRecord: Option<JournalRecord>,  // The page's if sb.freshestCU.Some?
-    rowResult: ChainResult,        // Can we parse this row and stitch the JournalRecord?
-    cumulativeResult: ChainResult, // only ChainSuccess if prior rows also succeed
-    cumulativeReadPtrs: seq<PagePointer>,    // All the PagePointers we've read up to this row.
-    cumulativeLsnMap: map<LSN, PagePointer> // Which PagePointer explains each LSN in result
+    journalRecord: Option<JournalRecord>,  // The page's if tj.freshestCU.Some?
+    rowResult: ChainResult,                // Can we parse this row and stitch the JournalRecord?
+    cumulativeResult: ChainResult          // only ChainSuccess if prior rows also succeed
     )
   {
-    function newReadPtrs() : seq<PagePointer> {
-      if sb.freshestPtr.None? then [] else [sb.freshestPtr.value]
-    }
     predicate WF() {
       && cumulativeResult.WF()
       // Note: WF doesn't say anything about values of cumulative fields; those get
       // defined in ValidSuccessorTo
 
-      && (journalRecord.Some? ==> sb.freshestPtr.Some?)
+      && (journalRecord.Some? ==> tj.freshestRec.Some?)
       && (journalRecord.Some? ==> journalRecord.value.WF())
 
       && (
-        if sb.freshestPtr.None?          // sb doesn't need anything
+        if tj.freshestRec.None?          // tj doesn't need anything
         then
           && journalRecord.None?
           && rowResult == ChainSuccess([], EmptyHistory)
         else if journalRecord.None?
-        then rowResult == ChainFailed // Expected journal record, didn't have one
+        then rowResult == ChainFailed // Expected initial journal record, didn't have one
         else
           if expectedEnd != journalRecord.value.messageSeq.seqEnd
             // and we're expecting a particular end value and record didn't stitch
           then rowResult == ChainFailed
-          else if journalRecord.value.messageSeq.seqEnd <= sb.boundaryLSN
+          else if journalRecord.value.messageSeq.seqEnd <= tj.boundaryLSN
             // parsed journal record but don't need any of its entries
           then rowResult == ChainSuccess([], EmptyHistory)
           else rowResult == ChainSuccess([journalRecord.value], journalRecord.value.messageSeq)
-            // NB that the PagePointer is in our readPtrs in either case, whether
-            // the journalRecord is in .records or not. TODO document where that's enforced.
         )
     }
 
@@ -171,40 +135,28 @@ module PagedJournalMod {
       journalRecord.value
     }
 
-    function readPtrs() : seq<PagePointer>
-      requires WF()
-    {
-      if sb.freshestPtr.Some? then [sb.freshestPtr.value] else []
-    }
-
-    function rowLsnMap() : map<LSN, PagePointer>
-      requires WF()
-    {
-      rowResult.lsnMap(sb.freshestPtr)
-    }
-
-    function priorSB() : Superblock
+    function priorTJ() : TruncatedJournal
       requires WF() && hasRecord()
     {
       if
         // We read a JournalRecord
-        && sb.freshestPtr.Some?
+        && tj.freshestRec.Some?
         // and needed more than it had to offer
-        && sb.boundaryLSN < journalRec().messageSeq.seqEnd
+        && tj.boundaryLSN < journalRec().messageSeq.seqEnd
         // and it had a prior pointer
-        && journalRec().priorPtr.Some?
+        && journalRec().priorRec.Some?
       then
-        journalRec().priorSB(sb)
+        tj.prior()
       else
-        Superblock(None, sb.boundaryLSN)
+        TruncatedJournal(None, tj.boundaryLSN)
     }
 
     predicate FirstRow()
       requires WF()
     {
-      || sb.freshestPtr.None?
+      || tj.freshestRec.None?
       || rowResult.ChainFailed?
-      || journalRec().messageSeq.seqEnd <= sb.boundaryLSN
+      || journalRec().messageSeq.seqEnd <= tj.boundaryLSN
     }
 
     predicate ValidSuccessorTo(prev: Option<ChainLookupRow>)
@@ -215,13 +167,11 @@ module PagedJournalMod {
         && prev.None?
         // Accumulators start out correctly
         && cumulativeResult == rowResult
-        && cumulativeReadPtrs == readPtrs()
-        && cumulativeLsnMap == rowLsnMap()
       else
         && prev.Some?
         && prev.value.WF()
         // superblock defines the row; those should link as expected
-        && prev.value.sb == priorSB()
+        && prev.value.tj == tj.prior()
         // if prior has a journalRec, its LSNs stitch seamlessly with this one
         && prev.value.expectedEnd == journalRec().messageSeq.seqStart
         // result success bit accumulates correctly
@@ -232,19 +182,6 @@ module PagedJournalMod {
             && prev.value.cumulativeResult.Concatable(rowResult)
             && cumulativeResult == prev.value.cumulativeResult.Concat(rowResult)
           )
-        // readPtrs accumulate correctly
-        && cumulativeReadPtrs == prev.value.cumulativeReadPtrs + readPtrs()
-        // lsnMaps accumulate correctly
-        // (The union is disjoint, but that knowledge requires an inductive proof)
-        && cumulativeLsnMap == MapUnionPreferA(prev.value.cumulativeLsnMap, rowLsnMap())
-    }
-
-    predicate RespectsDisk(storage: Storage)
-      requires WF()
-    {
-      sb.freshestPtr.Some? ==>
-        && sb.freshestPtr.value in storage
-        && journalRecord == Some(storage[sb.freshestPtr.value])
     }
   }
 
@@ -269,28 +206,20 @@ module PagedJournalMod {
       forall idx | 0 <= idx < |rows| :: Linked(idx)
     }
 
-    predicate RespectsDisk(storage: Storage)
-      requires WF()
-    {
-      forall idx | 0 <= idx < |rows| :: rows[idx].RespectsDisk(storage)
-    }
-
-    predicate Valid(storage: Storage) {
+    predicate Valid() {
       && WF()
       && Chained()
-      && RespectsDisk(storage)
     }
 
-    predicate ForSB(sb: Superblock)
+    predicate ForSB(tj: TruncatedJournal)
       requires WF()
     {
-      && Last(rows).sb == sb
+      && Last(rows).tj == tj
     }
 
-    predicate ValidForSB(storage: Storage, sb: Superblock) {
-      && WF()
-      && Valid(storage)
-      && ForSB(sb)
+    predicate ValidForSB(tj: TruncatedJournal) {
+      && Valid()
+      && ForSB(tj)
     }
 
     // Clients only care about the last row; the previous rows are all proof fodder.
@@ -314,12 +243,6 @@ module PagedJournalMod {
       last().cumulativeResult.interp
     }
 
-    function lsnMap() : map<LSN, PagePointer>
-      requires WF()
-    {
-      last().cumulativeLsnMap
-    }
-
     lemma SuccessTransitivity()
       requires WF() && success()
       ensures forall i | 0<=i<|rows| :: rows[i].cumulativeResult.ChainSuccess?;
@@ -333,22 +256,6 @@ module PagedJournalMod {
       {
         assert Linked(idx);
         idx := idx - 1;
-      }
-    }
-
-    lemma LsnMapDomain()
-      requires WF() && success()
-      ensures lsnMap().Keys == interp().LSNSet()
-    {
-      SuccessTransitivity();
-
-      var idx := 0;
-      while idx < |rows|
-        invariant idx <= |rows|
-        invariant forall i | 0 <= i < idx :: rows[i].cumulativeLsnMap.Keys == rows[i].cumulativeResult.interp.LSNSet()
-      {
-        assert Linked(idx);
-        idx := idx + 1;
       }
     }
 
@@ -373,12 +280,12 @@ module PagedJournalMod {
     }
   }
 
-  function EmptyChainLookup(sb: Superblock, expectedEnd: LSN) : (cl: ChainLookup)
-    requires sb.freshestPtr.None?
+  function EmptyChainLookup(tj: TruncatedJournal, expectedEnd: LSN) : (cl: ChainLookup)
+    requires tj.freshestRec.None?
     ensures cl.WF()
   {
     var emptyResult := ChainSuccess([], EmptyHistory);
-    var clrow := ChainLookupRow(sb, expectedEnd, None, emptyResult, emptyResult, [], EmptyLSNMap());
+    var clrow := ChainLookupRow(tj, expectedEnd, None, emptyResult, emptyResult);
     assert clrow.WF();
     ChainLookup([clrow])
   }
@@ -389,57 +296,44 @@ module PagedJournalMod {
   // expectedEnd is an Option, because, when the entry point ChainFrom calls
   // us, it doesn't know (or care) what expectedEnd value we need; we should
   // supply whatever the journalRec says.
-  function ChainFromRecursive(storage: Storage, sb: Superblock, expectedEnd: Option<LSN>) : (cl:ChainLookup)
-    ensures cl.ValidForSB(storage, sb)
+  function ChainFromRecursive(tj: TruncatedJournal, expectedEnd: Option<LSN>) : (cl:ChainLookup)
+    ensures cl.ValidForSB(tj)
     ensures expectedEnd.Some? ==> cl.last().expectedEnd == expectedEnd.value
     decreases if expectedEnd.Some? then 0 else 1, if expectedEnd.Some? then expectedEnd.value else 0
   {
     var expectedEndValue := match expectedEnd case Some(lsn) => lsn case None => 0;
-    if sb.freshestPtr.None?
+    if tj.freshestRec.None?
     then
-      var cl := EmptyChainLookup(sb, expectedEndValue);
+      var cl := EmptyChainLookup(tj, expectedEndValue);
       assert cl.WF();
-      assert cl.ValidForSB(storage, sb);
+      assert cl.ValidForSB(tj);
       cl
     else
-      var ptr := sb.freshestPtr.value;
-      if ptr !in storage
-      then
-        var row := ChainLookupRow(sb, expectedEndValue, None, ChainFailed, ChainFailed, [ptr], EmptyLSNMap());
-        var cl := ChainLookup([row]);
-        assert row.WF();
-        assert cl.WF();
-        assert cl.Valid(storage);
-        assert cl.ValidForSB(storage, sb);
-        cl
-      else
-        var journalRecord := storage[sb.freshestPtr.value];
-        if expectedEnd.Some? && expectedEndValue != journalRecord.messageSeq.seqEnd
+      var journalRecord := tj.freshestRec.value;
+
+        if && expectedEnd.Some?
+           && (journalRecord.messageSeq.EmptyHistory? || expectedEndValue != journalRecord.messageSeq.seqEnd)
           // we're expecting a particular end value and record didn't stitch
         then
-          var row := ChainLookupRow(sb, expectedEndValue, Some(journalRecord), ChainFailed, ChainFailed, [ptr], EmptyLSNMap());
+          var row := ChainLookupRow(tj, expectedEndValue, Some(journalRecord), ChainFailed, ChainFailed);
           var cl := ChainLookup([row]);
           assert cl.WF();
-          assert cl.ValidForSB(storage, sb);
           cl
-        else if journalRecord.messageSeq.seqEnd <= sb.boundaryLSN
+        else if journalRecord.messageSeq.seqEnd <= tj.boundaryLSN
         then // parsed journal record but don't need any of its entries
           var rowResult := ChainSuccess([], EmptyHistory);
-          var cl := ChainLookup([ChainLookupRow(sb, journalRecord.messageSeq.seqEnd, Some(journalRecord), rowResult, rowResult, [ptr], EmptyLSNMap())]);
+          var cl := ChainLookup([ChainLookupRow(tj, journalRecord.messageSeq.seqEnd, Some(journalRecord), rowResult, rowResult)]);
           assert cl.WF();
-          assert cl.ValidForSB(storage, sb);
           cl
         else
           var rowResult := ChainSuccess([journalRecord], journalRecord.messageSeq);
-          var remainder := ChainFromRecursive(storage, journalRecord.priorSB(sb), Some(journalRecord.messageSeq.seqStart));
+          var remainder := ChainFromRecursive(tj.prior(), Some(journalRecord.messageSeq.seqStart));
           var cl := ChainLookup(remainder.rows + [ChainLookupRow(
-            sb,
+            tj,
             journalRecord.messageSeq.seqEnd,
             Some(journalRecord),
             rowResult,
-            remainder.last().cumulativeResult.Concat(rowResult),
-            remainder.last().cumulativeReadPtrs+[ptr],
-            MapUnionPreferA(remainder.lsnMap(), rowResult.lsnMap(sb.freshestPtr))
+            remainder.last().cumulativeResult.Concat(rowResult)
           )]);
           assert cl.Chained() by {
             forall idx | 0 <= idx < |cl.rows| ensures cl.Linked(idx) {
@@ -449,7 +343,6 @@ module PagedJournalMod {
             }
           }
           assert cl.WF();
-          assert cl.ValidForSB(storage, sb);
           cl
   }
 
@@ -465,10 +358,10 @@ module PagedJournalMod {
     }
   }
 
-  lemma UniqueChainLookup(storage: Storage, cla: ChainLookup, clb: ChainLookup)
-    requires cla.Valid(storage)
-    requires clb.Valid(storage)
-    requires cla.last().sb == clb.last().sb
+  lemma UniqueChainLookup(cla: ChainLookup, clb: ChainLookup)
+    requires cla.Valid()
+    requires clb.Valid()
+    requires cla.last().tj == clb.last().tj
     requires cla.last().expectedEnd == clb.last().expectedEnd
     ensures cla == clb
     decreases |cla.rows|
@@ -480,24 +373,24 @@ module PagedJournalMod {
     if 1 < |cla.rows| {
       ChainedPrior(cla);
       ChainedPrior(clb);
-      UniqueChainLookup(storage, cla.DropLast(), clb.DropLast()); // recurse
+      UniqueChainLookup(cla.DropLast(), clb.DropLast()); // recurse
     }
   }
 
-  function {:opaque} ChainFrom(storage: Storage, sb: Superblock) : (cl:ChainLookup)
-    ensures cl.ValidForSB(storage, sb)
+  function {:opaque} ChainFrom(tj: TruncatedJournal) : (cl:ChainLookup)
+    ensures cl.Valid()
     ensures cl.Complete()
-    ensures forall ocl:ChainLookup | ocl.ValidForSB(storage, sb) && ocl.Complete() :: ocl == cl
+    ensures forall ocl:ChainLookup | ocl.Valid() && ocl.Complete() :: ocl == cl // TODO um no must share tj
   {
-    var cl := ChainFromRecursive(storage, sb, None);
-    assert forall ocl:ChainLookup | ocl.ValidForSB(storage, sb) && ocl.Complete() :: ocl == cl by {
-      forall ocl:ChainLookup | ocl.ValidForSB(storage, sb) && ocl.Complete() ensures ocl == cl {
+    var cl := ChainFromRecursive(tj, None);
+    assert forall ocl:ChainLookup | ocl.Valid() && ocl.Complete() :: ocl == cl by {
+      forall ocl:ChainLookup | ocl.Valid() && ocl.Complete() ensures ocl == cl {
       // TODO(jonh): clean up unneeded proof
         assert cl.Complete();
         assert ocl.Complete();
         if cl.last().hasRecord() {
-          assert cl.last().sb.freshestPtr.Some?;
-          assert ocl.last().sb.freshestPtr.Some?;
+          assert cl.last().tj.freshestRec.Some?;
+          assert ocl.last().tj.freshestRec.Some?;
           assert cl.last().journalRecord.Some?;
           assert ocl.last().journalRecord.Some?;
 
@@ -520,7 +413,7 @@ module PagedJournalMod {
             cl.last().expectedEnd;
           }
         }
-        UniqueChainLookup(storage, cl, ocl);
+        UniqueChainLookup(cl, ocl);
       }
     }
     cl
@@ -554,11 +447,8 @@ module PagedJournalMod {
     unmarshalledTail: seq<KeyedMessage>,
       // The rest of the in-memory journal
 
-    marshalledLookup: ChainLookup
-      // We imagine that the journal can keep track of the entire mapping from LSN to Ptrs
-      // (which we're grabbing here as the cumulativeLsnMap).
-      // That's not really how the impl will work; it'll maintain some sort of summary, and
-      // we'll refine from the disk state to get this field.
+    truncatedJournal: TruncatedJournal
+      // The linked list of journal pages
   )
   {
     // A "public" method for Program to inquire where Journal begins
@@ -573,81 +463,29 @@ module PagedJournalMod {
 
     predicate WF() {
       && boundaryLSN <= persistentLSN <= cleanLSN <= marshalledLSN
-      && marshalledLookup.WF()
-      && marshalledLookup.success()
-      && marshalledLookup.interp().CanFollow(boundaryLSN)
-      && marshalledLookup.interp().SeqEndFor(boundaryLSN) == marshalledLSN
-    }
-
-    function FreshestMarshalledPtr() : Option<PagePointer>
-      requires WF()
-    {
-      marshalledLookup.LsnMapDomain();
-
-      if marshalledLSN == boundaryLSN
-      then None
-      else Some(marshalledLookup.lsnMap()[marshalledLSN-1])
-    }
-
-    // This is the superblock that v would use if it all the marshalled stuff were clean
-    function CurrentSuperblock() : Superblock
-      requires WF()
-    {
-      Superblock(FreshestMarshalledPtr(), boundaryLSN)
-    }
-
-    function lsnMap() : map<LSN, PagePointer>
-      requires WF()
-    {
-      marshalledLookup.last().cumulativeLsnMap
     }
   }
 
   datatype InitSkolems = InitSkolems(sbJournalRec: JournalRecord)
 
-  function MkfsSuperblock() : Superblock
+  function MkfsTruncatedJournal() : TruncatedJournal
   {
-    Superblock(None, 0)
+    TruncatedJournal(None, 0)
   }
 
-  predicate Init(v: Variables, sb: Superblock, storage: Storage, sk: InitSkolems)
+  predicate Init(v: Variables, tj: TruncatedJournal, sk: InitSkolems)
   {
-    // Can't proceed if there's a freshestPtr but there's not a journal page
-    // there in the storage.
-    && sb.freshestPtr.Some? ==> (
-      && sb.freshestPtr.value in storage
-      && storage[sb.freshestPtr.value] == sk.sbJournalRec
-      )
-
     // Figure out where journal ends
     && var lastLSN :=
-      if sb.freshestPtr.None?
+      if tj.freshestRec.None?
       then
-        sb.boundaryLSN
+        tj.boundaryLSN
       else
         sk.sbJournalRec.messageSeq.seqEnd;
 
-    && v.boundaryLSN == sb.boundaryLSN == 0
+    && v.boundaryLSN == tj.boundaryLSN == 0
     && v.persistentLSN == v.cleanLSN == v.marshalledLSN == lastLSN == 0
     && v.unmarshalledTail == []
-
-    // TODO this fails WF! And will require storage to decode
-    && v.marshalledLookup == EmptyChainLookup(Superblock(None, 0), 0)
-  }
-
-  // Recovery coordination
-  predicate MessageSeqMatchesJournalAt(v: Variables, puts: MsgHistory)
-    requires v.WF()
-    requires puts.WF()
-  {
-    // NB elsewhere in the state machine, we rely only on v.marshalledLookup
-    // containing an accurate mapping between LSNs and Ptrs; here, we care about
-    // the message seq interpretation as well. So the refined implementation, in
-    // addition to maintaining location information, will need to fault in a
-    // range of marshalled pages to confirm these contents match during recovery.
-    // NB we only consider the marshalledLookup because, during recovery, there
-    // had best not be anything in the unmarshalledTail!
-    && v.marshalledLookup.interp().IncludesSubseq(puts)
   }
 
   // advances tailLSN forward by adding a message
@@ -666,132 +504,37 @@ module PagedJournalMod {
     else MsgHistory(map i: LSN | start <= i < end :: v.unmarshalledTail[i - start], start, end)
   }
 
-  // advances marshalledLSN forward by marshalling a batch of messages into a dirty storage page
-  predicate AdvanceMarshalled(v: Variables, v': Variables, storage: Storage, storage': Storage, newPtr: PagePointer)
-  {
-    && v.WF()
-
-    // Not allowed to append empty journal records.
-    && 0 < |v.unmarshalledTail|
-
-    // newPtr is an unused PagePointer.
-    // That could be because the impl has freshly reserved a chunk of Ptrs from the outer
-    // program, or because it's using up a PagePointer from a prior reserved chunk. The impl will
-    // batch allocations so it can avoid needing to rewrite the marshaled allocation before
-    // commiting a fresh superblock (on sync). Thus "unused" may be computed as "reserved
-    // but known not to be in use in the current JournalChain".
-    && newPtr !in ChainFrom(storage, v.CurrentSuperblock()).last().cumulativeReadPtrs
-
-    // Marshal and write the current record out into the storage. (This doesn't issue
-    // a disk write, it just dirties a page.)
-    && var priorPtr := (v.marshalledLookup.LsnMapDomain(); if v.marshalledLSN == v.boundaryLSN then None else Some(v.lsnMap()[v.marshalledLSN-1]));
-    && var newRec := JournalRecord(TailToMsgSeq(v), priorPtr);
-    && storage' == storage[newPtr := newRec]
-
-    // Record the changes to the marshalled, unmarshalled regions, and update the allocation.
-    && v' == v.(
-      // Open a new, empty record to absorb future journal Appends
-      marshalledLSN := v.unmarshalledLSN(),
-      unmarshalledTail := [],
-      marshalledLookup := v'.marshalledLookup  // Tautology to defer this constraint to next predicate
-      )
-    // constructive: (map lsn:LSN | 0 <= lsn < v.unmarshalledLSN() :: if lsn < v.marshalledLSN then v.marshalledLookup[lsn] else newPtr),
-    // predicate:
-    && FullStorage(storage)
-    &&
-      //reveal_ChainFrom();
-      v'.marshalledLookup == ChainFrom(storage', Superblock(Some(newPtr), v.boundaryLSN))
-  }
-
-  // advances cleanLSN forward by learning that the storage has written back a contiguous
-  // sequence of pages starting at last cleanLSN
-  predicate AdvanceClean(v: Variables, v': Variables, storage: Storage, storage': Storage, newClean: nat)
-  {
-    && v.WF()
-    && v.cleanLSN < newClean <= v.marshalledLSN
-
-    // true conjunct here stands for a cache-clean condition from a layer below.
-    // TODO(jonh) Suggests maybe we should remove this state & transition from this model.
-    && true
-
-    && v' == v.(cleanLSN := newClean)
-    && storage' == storage
-  }
-
-  predicate Reallocate(v: Variables, v': Variables)
-  {
-    // TODO Allocation isn't what we want, yet. It's tight, so we have to write
-    // a new allocation table every time we change the superblock. That's no
-    // good!
-    && false // does something with allocation table?
-  }
-
-  function FreshestCleanPtr(v: Variables) : Option<PagePointer>
-    requires v.WF()
-  {
-    v.marshalledLookup.LsnMapDomain();
-
-    if v.cleanLSN == v.boundaryLSN
-    then None
-    else Some(v.lsnMap()[v.cleanLSN-1])
-  }
-
   // Agrees to advance persistentLSN (to cleanLSN) and firstLSN (to newBoundary, coordinated
   // with BeTree) as part of superblock writeback.
-  predicate CommitStart(v: Variables, v': Variables, storage: Storage, sb: Superblock, newBoundaryLSN: LSN)
+  predicate CommitStart(v: Variables, v': Variables, tj: TruncatedJournal, newBoundaryLSN: LSN)
   {
     && v.WF()
-    // This is the stuff we'll get to garbage collect when the sb commit completes.
+    // This is the stuff we'll get to garbage collect when the tj commit completes.
     && v.boundaryLSN <= newBoundaryLSN // presumably provable from Inv
 
-    // These are the LSNs whose syncs will complete when the sb commit completes.
+    // These are the LSNs whose syncs will complete when the tj commit completes.
     && v.persistentLSN <= v.cleanLSN  // presumably provable from Inv
 
     // everything we're proposing to commit is cleaned
     && newBoundaryLSN <= v.cleanLSN
 
     // This is the superblock that's going to become persistent.
-    && sb == Superblock(FreshestCleanPtr(v), newBoundaryLSN)
+    // TODO(jonh): this is too strong; we need to separate clean from marshalled, I think, to
+    // allow prefix commits.
+    && tj == v.truncatedJournal
     && v' == v
   }
 
   // Learns that coordinated superblock writeback is complete; updates persistentLSN & firstLSN.
-  predicate CommitComplete(s: Variables, s': Variables, storage: Storage, sb: Superblock)
+  predicate CommitComplete(s: Variables, s': Variables, tj: TruncatedJournal)
   {
     && s.WF()
 
-    && s'.boundaryLSN == sb.boundaryLSN
+    && s'.boundaryLSN == tj.boundaryLSN
 
-    // Update s'.persistentLSN so that it reflects a persisted LSN (something in the last block,
-    // ideally the last LSN in that block). NB This gives impl freedom to not
-    // record the latest persistent LSN in the freshestPtr block, which would be
-    // kind of dumb (it would hold up syncs for no reason), but not unsafe.
-    && (if sb.freshestPtr.None?
-        then s'.persistentLSN == sb.boundaryLSN
-        else
-          && s'.persistentLSN - 1 in s.lsnMap()
-          && s.lsnMap()[s'.persistentLSN - 1] == sb.freshestPtr.value
-        )
     && s'.cleanLSN == s.cleanLSN
     && s'.marshalledLSN == s.marshalledLSN
     && s'.unmarshalledTail == s.unmarshalledTail
-    && s'.marshalledLookup == ChainFrom(storage, sb)
-  }
-
-  datatype Skolem =
-    | AdvanceMarshalledStep(newPtr: PagePointer)
-    | AdvanceCleanStep(newClean: nat)
-
-  predicate Internal(s: Variables, s': Variables, storage: Storage, storage': Storage, sk: Skolem) {
-    match sk {
-      case AdvanceMarshalledStep(newPtr) => AdvanceMarshalled(s, s', storage, storage', newPtr)
-      case AdvanceCleanStep(newClean) => AdvanceClean(s, s', storage, storage', newClean)
-//      case _ => false
-    }
-  }
-
-  function Alloc(s: Variables) : set<PagePointer> {
-    {} // TODO
   }
 }
 
