Splinter/Paged/PagedSystem.i.dfy
@@ -1,0 +1,476 @@
+// Copyright 2018-2021 VMware, Inc., Microsoft Inc., Carnegie Mellon University, ETH Zurich, and University of Washington
+// SPDX-License-Identifier: BSD-2-Clause
+
+include "../../Spec/MapSpec.s.dfy"
+include "../../lib/Base/KeyType.s.dfy"
+include "../../lib/Base/MapRemove.s.dfy"
+include "../CoordinationLayer/MsgHistory.i.dfy"
+
+abstract module JournalIfc {
+  import opened Options
+  import opened MsgHistoryMod
+  import opened StampedMapMod // LSN TODO(jonh): move
+
+  type PersistentJournal(==,!new)
+  type EphemeralJournal(==,!new)
+
+  predicate PWF(pj: PersistentJournal)
+  predicate EWF(ej: EphemeralJournal)
+
+  function Mkfs() : PersistentJournal
+
+  function LoadJournal(pj: PersistentJournal) : EphemeralJournal
+
+  // TODO rename PJournalSeqEnd, I guess
+  function JournalSeqEnd(pj: PersistentJournal) : Option<LSN>
+
+  function EJournalSeqEnd(ej: EphemeralJournal) : Option<LSN>
+
+  predicate JournalIncludesSubseq(ej: EphemeralJournal, msgs: MsgHistory)
+    requires EWF(ej)
+    requires msgs.WF()
+
+  function JournalConcat(ej: EphemeralJournal, msgs: MsgHistory) : EphemeralJournal
+    requires EWF(ej)
+    requires msgs.WF()
+    requires msgs.EmptyHistory? || EJournalSeqEnd(ej).None? || msgs.CanFollow(EJournalSeqEnd(ej).value)
+    ensures EWF(JournalConcat(ej, msgs))
+
+  predicate JournalCanFreeze(ej: EphemeralJournal, startLsn: LSN, endLsn: LSN)
+
+  function JournalFreeze(ej: EphemeralJournal, startLsn: LSN, endLsn: LSN) : PersistentJournal
+    requires EWF(ej);
+    requires JournalCanFreeze(ej, startLsn, endLsn)
+
+  predicate CanDiscardOld(ej: EphemeralJournal, lsn: LSN)
+
+  function DiscardOld(ej: EphemeralJournal, lsn: LSN) : EphemeralJournal
+    requires EWF(ej)
+    requires CanDiscardOld(ej, lsn)
+}
+
+module AbstractJournal refines JournalIfc {
+  type PersistentJournal = MsgHistory
+  type EphemeralJournal = MsgHistory
+
+  predicate PWF(pj: PersistentJournal) {
+    pj.WF()
+  }
+
+  predicate EWF(ej: EphemeralJournal) {
+    ej.WF()
+  }
+
+  function JournalSeqEnd(pj: PersistentJournal) : Option<LSN>
+  {
+    if pj.MsgHistory? then Some(pj.seqEnd) else None
+  }
+
+  predicate JournalIncludesSubseq(ej: EphemeralJournal, msgs: MsgHistory)
+    //requires EWF(ej)
+    //requires msg.WF()
+  {
+    ej.IncludesSubseq(msgs)
+  }
+
+  function EJournalSeqEnd(ej: EphemeralJournal) : Option<LSN>
+  {
+    if ej.MsgHistory? then Some(ej.seqEnd) else None
+  }
+
+  function JournalConcat(ej: EphemeralJournal, msgs: MsgHistory) : EphemeralJournal
+    //requires EWF(ej)
+    //requires msg.WF()
+    //requires msgs.EmptyHistory? || EJournalSeqEnd(ej).None? || msgs.CanFollow(EJournalSeqEnd(ej).value)
+    //ensures EWF(JournalConcat(ej, msgs))
+  {
+    ej.Concat(msgs)
+  }
+
+  predicate CanDiscardOld(ej: EphemeralJournal, lsn: LSN)
+  {
+    ej.CanDiscardTo(lsn)
+  }
+
+  function DiscardOld(ej: EphemeralJournal, lsn: LSN) : EphemeralJournal
+    // requires EWF(ej)
+    // requires CanDiscardOld(ej, lsn)
+  {
+    ej.DiscardOld(lsn)
+  }
+
+  predicate JournalCanFreeze(ej: EphemeralJournal, startLsn: LSN, endLsn: LSN)
+  {
+    // TODO(jonh): journal impl tells us what it can freeze.
+    // Here we pretend we can freeze anything in the journal
+    || startLsn==endLsn
+    || (
+      && ej.MsgHistory?
+      && ej.seqStart <= startLsn < endLsn <= ej.seqStart
+      )
+  }
+
+  function JournalFreeze(ej: EphemeralJournal, startLsn: LSN, endLsn: LSN) : PersistentJournal
+    // requires EWF(ej);
+    // requires JournalCanFreeze(ej, startLsn, endLsn)
+  {
+    if startLsn==endLsn
+    then EmptyHistory
+    else
+      ej.DiscardOld(startLsn).DiscardRecent(endLsn)
+  }
+}
+
+// module PagedJournal refines JournalIfc {
+// }
+
+module CoordinatorMod(journalMod: JournalIfc)  {
+  import opened Options
+  import opened MapRemove_s
+  import opened StampedMapMod
+  import opened CrashTolerantMapSpecMod
+  import opened MsgHistoryMod
+  import opened KeyType
+  import opened ValueMessage
+  import opened FullKMMapMod
+
+  import Async = CrashTolerantMapSpecMod.async
+
+  // TODO(jonh): plug in PagedMap here. Right now only exploring journal.
+  type MapAdt = StampedMapMod.StampedMap
+  type Journal = journalMod.PersistentJournal
+
+  function MapAdtMkfs() : MapAdt {
+    StampedMapMod.Empty()
+  }
+
+  datatype DiskImage = DiskImage(
+    mapadt: MapAdt,
+    journal: Journal
+    )
+  {
+    predicate WF() { true }
+
+    function SeqEnd() : LSN
+    {
+      if journalMod.JournalSeqEnd(journal).Some? then journalMod.JournalSeqEnd(journal).value else mapadt.seqEnd
+    }
+
+    predicate CompletesSync(lsn: LSN)
+    {
+      lsn < SeqEnd()
+    }
+  }
+  
+  type SyncReqs = map<CrashTolerantMapSpecMod.SyncReqId, LSN>
+  
+  datatype Ephemeral =
+    | Unknown
+    | Known(
+      progress: Async.EphemeralState,
+      syncReqs: SyncReqs,
+
+      mapadt: MapAdt,
+      journal: journalMod.EphemeralJournal,
+
+      frozenMap: Option<MapAdt>
+    )
+  {
+    predicate WF() {
+      Known? ==> (
+        && journalMod.EWF(journal)
+      )
+    }
+  }
+
+  function MkfsDiskImage() : DiskImage
+  {
+    DiskImage(MapAdtMkfs(), journalMod.Mkfs())
+  }
+
+  // TODO(jonh): maybe this is a parameterized type we can reuse in CMJ & here?
+  // Actually, maybe we should parameterize the entire module and plug in these
+  // paged implementations! I'll start with it concrete though.
+  datatype Variables = Variables(
+    persistentImage: DiskImage,
+    ephemeral: Ephemeral,
+    inFlightImage: Option<DiskImage>
+  )
+  {
+    predicate WF()
+    {
+      && persistentImage.WF()
+      && (ephemeral.Known? ==> ephemeral.WF())
+      && (inFlightImage.Some? ==> inFlightImage.value.WF())
+    }
+
+    predicate Mkfs()
+    {
+      && persistentImage == MkfsDiskImage()
+      && ephemeral.Unknown?
+      && inFlightImage.None?
+    }
+  }
+    
+  predicate LoadEphemeralFromPersistent(v: Variables, v': Variables, uiop : UIOp)
+  {
+    && uiop.NoopOp?
+    && v.ephemeral.Unknown?
+    && v' == v.(ephemeral := Known(
+      Async.InitEphemeralState(),
+      map[],  // syncReqs
+      v.persistentImage.mapadt,
+      journalMod.LoadJournal(v.persistentImage.journal),
+      None  // frozen map
+      ))
+  }
+
+  // The ephemeral map and ephemeral journal are at the same lsn, which only happens
+  // after recovery has "caught the map up" to the journal.
+  predicate MapIsFresh(v: Variables)
+  {
+    && v.WF()
+    && v.ephemeral.Known?
+    && var jend := journalMod.JournalSeqEnd(v.persistentImage.journal);
+      (jend.Some? ==> jend.value == v.ephemeral.mapadt.seqEnd)
+  }
+
+  function NextLSN(v: Variables) : LSN
+    requires v.ephemeral.Known?
+  {
+    v.ephemeral.mapadt.seqEnd
+  }
+
+  // Move some journal state into the map to make it (closer to) fresh
+  predicate Recover(v: Variables, v': Variables, uiop : UIOp, puts:MsgHistory)
+  {
+    && uiop.NoopOp?
+    && v.WF()
+    && v.ephemeral.Known?
+    && !MapIsFresh(v)
+    && v'.WF()
+
+    && puts.WF()
+    && puts.CanFollow(v.ephemeral.mapadt.seqEnd)
+    && journalMod.JournalIncludesSubseq(v.ephemeral.journal, puts)
+
+    // NB that Recover can interleave with mapadt steps (the Betree
+    // reorganizing its state, possibly flushing stuff out to disk).
+    && v' == v.(ephemeral := v.ephemeral.(mapadt := MapPlusHistory(v.ephemeral.mapadt, puts)))
+  }
+
+  predicate AcceptRequest(v: Variables, v': Variables, uiop : UIOp)
+  {
+    && v.ephemeral.Known?
+    && uiop.OperateOp?
+    && uiop.baseOp.RequestOp?
+    && uiop.baseOp.req !in v.ephemeral.progress.requests
+    && v' == v.(ephemeral := v.ephemeral.(progress := v.ephemeral.progress.(
+        requests := v.ephemeral.progress.requests + {uiop.baseOp.req})))
+  }
+
+  predicate Query(v: Variables, v': Variables, uiop : UIOp)
+  {
+    && MapIsFresh(v)
+    && uiop.OperateOp?
+    && uiop.baseOp.ExecuteOp?
+    && uiop.baseOp.req.input.GetInput? // ensures that the uiop translates to a Get op
+    && uiop.baseOp.reply.output.GetOutput?
+    && uiop.baseOp.req in v.ephemeral.progress.requests
+    && uiop.baseOp.reply.id == uiop.baseOp.req.id
+
+    && uiop.baseOp.req in v.ephemeral.progress.requests
+    && uiop.baseOp.reply !in v.ephemeral.progress.replies
+    && var key := uiop.baseOp.req.input.key;
+    && var value := uiop.baseOp.reply.output.value;
+    && assert AnyKey(key);
+    && value == v.ephemeral.mapadt.mi[key].value
+    && v' == v.(ephemeral := v.ephemeral.(progress := v.ephemeral.progress.(
+        requests := v.ephemeral.progress.requests - {uiop.baseOp.req},
+        replies := v.ephemeral.progress.replies + {uiop.baseOp.reply}
+      )))
+  }
+
+  predicate Put(v: Variables, v': Variables, uiop : UIOp)
+  {
+    // Here we're not allowing puts until MapIsFresh, and then maintaining that
+    // invariant. We could alternately allow puts to run ahead, and then just
+    // let Queries be delayed until Recover catches up the mapadt.
+    // I'm modeling it this way because this matches the phase-driven behavior
+    // (recover, then be done recovering until next crash) we expect the real
+    // implementation to maintain.
+    && MapIsFresh(v)
+
+    && uiop.OperateOp?
+    && uiop.baseOp.ExecuteOp?
+    && uiop.baseOp.req.input.PutInput? // ensures that the uiop translates to a put op
+    && uiop.baseOp.reply.output.PutOutput?
+    && uiop.baseOp.req in v.ephemeral.progress.requests
+    && uiop.baseOp.reply.id == uiop.baseOp.req.id
+    && uiop.baseOp.reply !in v.ephemeral.progress.replies
+
+    && var key := uiop.baseOp.req.input.key;
+    && var val := uiop.baseOp.req.input.value;
+
+    && var singleton := MsgHistoryMod.Singleton(NextLSN(v), KeyedMessage(key, Define(val)));
+
+    && v.WF()
+    && v' == v.(ephemeral := v.ephemeral.(
+          journal := journalMod.JournalConcat(v.ephemeral.journal, singleton),
+          mapadt := MapPlusHistory(v.ephemeral.mapadt, singleton),
+          // Frozen stuff unchanged here.
+          progress := v.ephemeral.progress.(
+            requests := v.ephemeral.progress.requests - {uiop.baseOp.req},
+            replies := v.ephemeral.progress.replies + {uiop.baseOp.reply}
+          )
+      ))
+  }
+
+  predicate DeliverReply(v: Variables, v': Variables, uiop : UIOp)
+  {
+    && v.ephemeral.Known?
+    && uiop.OperateOp?
+    && uiop.baseOp.ReplyOp?
+    && uiop.baseOp.reply in v.ephemeral.progress.replies
+    && v' == v.(ephemeral := v.ephemeral.(progress := v.ephemeral.progress.(
+        replies := v.ephemeral.progress.replies - {uiop.baseOp.reply})))
+  }
+
+  // Journal Internal steps (writing stuff out to disk, for example)
+  // and Betree Internal steps (writing stuff to disk, flushing and compacting,
+  // which create new blocks in cache and rearrange the indirection table)
+  // all look like stutters at this layer.
+
+  // predicate JournalInternal(v: Variables, v': Variables, uiop : UIOp, cacheOps: CacheIfc.Ops, sk: JournalMachineMod.Skolem)
+  // predicate SplinterTreeInternal(v: Variables, v': Variables, uiop : UIOp, cacheOps: CacheIfc.Ops, sk: SplinterTreeMachineMod.Skolem)
+
+  predicate ReqSync(v: Variables, v': Variables, uiop : UIOp)
+  {
+    && uiop.ReqSyncOp?
+    && MapIsFresh(v) // Actually, v.ephemeral.Known? is sufficient here.
+    && v'.ephemeral.Known?
+    && uiop.syncReqId !in v.ephemeral.syncReqs
+    // NB that the label for a sync in the table is the LSN AFTER the last write
+    && v' == v.(ephemeral := v.ephemeral.(
+        syncReqs := v.ephemeral.syncReqs[uiop.syncReqId := NextLSN(v)]
+      ))
+  }
+
+  predicate ReplySync(v: Variables, v': Variables, uiop : UIOp)
+  {
+    && uiop.ReplySyncOp?
+    && MapIsFresh(v) // Actually, v.ephemeral.Known? is sufficient here.
+    && uiop.syncReqId in v.ephemeral.syncReqs
+    && v.persistentImage.CompletesSync(v.ephemeral.syncReqs[uiop.syncReqId]) // sync lsn is persistent
+    && v' == v.(ephemeral := v.ephemeral.(
+        syncReqs := MapRemove1(v.ephemeral.syncReqs, uiop.syncReqId)
+      ))
+  }
+
+  predicate FreezeMapAdt(v: Variables, v': Variables, uiop : UIOp)
+  {
+    && uiop.NoopOp?
+    && v.WF()
+    && v.ephemeral.Known?
+    // Copy the current map into the frozen one, deleting whatever was
+    // frozen.
+    // TODO this should cause mischief if a Commit is in progress. Does it?
+    && v' == v.(ephemeral := v.ephemeral.(frozenMap := Some(v.ephemeral.mapadt)))
+  }
+
+  predicate CommitStart(v: Variables, v': Variables, uiop : UIOp, endJournal: LSN)
+  {
+    && uiop.NoopOp?
+    && v.WF()
+    && v.ephemeral.Known?
+    && v.inFlightImage.None?
+
+    && v.ephemeral.frozenMap.Some?
+    && var startJournal := v.ephemeral.frozenMap.value.seqEnd;
+    // Frozen map can't go backwards vs persistent map, lest we end up with
+    // a gap to the ephemeral journal start.
+    && v.persistentImage.mapadt.seqEnd <= startJournal
+    // And of course there should be no way for it to have passed the ephemeral map!
+    && startJournal <= v.ephemeral.mapadt.seqEnd
+    && journalMod.JournalCanFreeze(v.ephemeral.journal, startJournal, endJournal)
+
+    && v'.inFlightImage.Some?
+    && v' == v.(inFlightImage := Some(DiskImage(
+        v.ephemeral.frozenMap.value,
+        journalMod.JournalFreeze(v.ephemeral.journal, startJournal, endJournal))))
+  }
+
+  predicate CommitComplete(v: Variables, v': Variables, uiop : UIOp)
+  {
+    && v.inFlightImage.Some?
+    && var ifImage := v.inFlightImage.value;
+
+    && uiop.SyncOp?
+    && MapIsFresh(v) // Actually, v.ephemeral.Known? is sufficient here.
+
+    // TODO(jonh): this had better be an invariant, but if it's not, we're
+    // gonna have a weird liveness/crash recovery bug. Confirm that'll show up in
+    // proof.
+    && journalMod.CanDiscardOld(v.ephemeral.journal, ifImage.mapadt.seqEnd)
+
+    // pruning below is nonsense without this, but "luckily" this is an invariant:
+//    && JournalCanDiscardTo(v.ephemeral.journal, ifImage.mapadt.seqEnd)
+
+    // Now that the disk journal is updated, we need to behead the
+    // ephemeral journal, since interpretation want to CanFollow it
+    // onto the persistent mapadt.
+    && var j' := journalMod.DiscardOld(v.ephemeral.journal, ifImage.mapadt.seqEnd);
+
+    && v' == v.(
+        persistentImage := ifImage,
+        ephemeral := v.ephemeral.(journal := j'),
+        // Update journal, mapadt here if modeling clean, frozen
+        inFlightImage := None)
+  }
+
+  predicate Crash(v: Variables, v': Variables, uiop : UIOp)
+  {
+    && uiop.CrashOp?
+    && v' == v.(ephemeral := Unknown, inFlightImage := None)
+  }
+
+  datatype Step =
+    | LoadEphemeralFromPersistentStep()
+    | RecoverStep(puts:MsgHistory)
+    | AcceptRequestStep()
+    | QueryStep()
+    | PutStep()
+    | DeliverReplyStep()
+//    | JournalInternalStep()
+//    | SplinterTreeInternalStep()
+    | ReqSyncStep()
+    | ReplySyncStep()
+    | FreezeJournalStep(newFrozenLSN: LSN)
+    | FreezeMapAdtStep()
+    | CommitStartStep(seqBoundary: LSN)
+    | CommitCompleteStep()
+    | CrashStep()
+
+  predicate NextStep(v: Variables, v': Variables, uiop : UIOp, step: Step) {
+    match step {
+      case LoadEphemeralFromPersistentStep() => LoadEphemeralFromPersistent(v, v', uiop)
+      case RecoverStep(puts) => Recover(v, v', uiop, puts)
+      case AcceptRequestStep() => AcceptRequest(v, v', uiop)
+      case QueryStep() => Query(v, v', uiop)
+      case PutStep() => Put(v, v', uiop)
+//      case JournalInternalStep(sk) => JournalInternal(v, v', uiop, cacheOps, sk)
+//      case SplinterTreeInternalStep(sk) => SplinterTreeInternal(v, v', uiop, cacheOps, sk)
+      case DeliverReplyStep() => DeliverReply(v, v', uiop)
+      case ReqSyncStep() => ReqSync(v, v', uiop)
+      case ReplySyncStep() => ReplySync(v, v', uiop)
+      case FreezeMapAdtStep() => FreezeMapAdt(v, v', uiop)
+      case CommitStartStep(seqBoundary) => CommitStart(v, v', uiop, seqBoundary)
+      case CommitCompleteStep() => CommitComplete(v, v', uiop)
+      case CrashStep() => Crash(v, v', uiop)
+    }
+  }
+
+  predicate Next(v: Variables, v': Variables, uiop: UIOp) {
+    exists step :: NextStep(v, v', uiop, step)
+  }
+}
